theories/MetaTheory/Confluence.v
@@ -8,38 +8,53 @@ From Metaprog.MetaTheory Require Export Reduction.
 (** * Parallel reduction. *)
 (***********************************************************************)
 
+#[local] Reserved Notation "Σ |- t >> u"
+  (at level 50, no associativity, t at next level, u at next level).
+
 Unset Elimination Schemes.
 
 (** Parallel reduction relation. *)
-Inductive pred1 {s} : term s -> term s -> Prop :=
+Inductive pred1 {s} (Σ : evar_map) : term s -> term s -> Prop :=
 
 (** Beta-reduction rule. *)
-| pred1_app_beta x ty ty' body body' arg arg' args args' :
-    pred1 ty ty' ->
-    pred1 body body' ->
-    pred1 arg arg' ->
-    All2 pred1 args args' ->
-    pred1 (TApp (TLam x ty body) (arg :: args)) (TApp (body'[x := arg']) args')
+| pred1_app_beta x ty body body' arg arg' args args' :
+    Σ |- body >> body' ->
+    Σ |- arg >> arg' ->
+    All2 (pred1 Σ) args args' ->
+    Σ |- TApp (TLam x ty body) (arg :: args) >> TApp (body'[x := arg']) args'
+
+(** Evar expansion rule. *)
+| pred1_evar_expand ev ty def :
+    Σ ev = Some (mk_evar_entry ty (Some def)) ->
+    Σ |- TEvar ev >> wk def
 
 (** Congruence rules. *)
 
 | pred1_type :
-    pred1 TType TType
+    Σ |- TType >> TType
 
 | pred1_var i :
-    pred1 (TVar i) (TVar i)
+    Σ |- TVar i >> TVar i
 
 | pred1_lam x ty ty' body body' :
-    pred1 ty ty' -> pred1 body body' -> pred1 (TLam x ty body) (TLam x ty' body')
+    Σ |- ty >> ty' ->
+    Σ |- body >> body' ->
+    Σ |- TLam x ty body >> TLam x ty' body'
 
 | pred1_prod x a a' b b' :
-    pred1 a a' -> pred1 b b' -> pred1 (TProd x a b) (TProd x a' b')
+    Σ |- a >> a' ->
+    Σ |- b >> b' ->
+    Σ |- TProd x a b >> TProd x a' b'
 
 | pred1_app f f' args args' :
-    pred1 f f' -> All2 pred1 args args' -> pred1 (TApp f args) (TApp f' args')
+    Σ |- f >> f' ->
+    All2 (pred1 Σ) args args' ->
+    Σ |- TApp f args >> TApp f' args'
 
 | pred1_evar ev :
-    pred1 (TEvar ev) (TEvar ev).
+    Σ |- TEvar ev >> TEvar ev
+
+where "Σ |- t >> u" := (pred1 Σ t u).
 
 Set Elimination Schemes.
 
@@ -47,35 +62,41 @@ Derive Signature for pred1.
 
 (** Induction principle for [pred1]. We can't use Rocq's default induction principle
     because [pred1] is nested over [All2]. *)
-Lemma pred1_ind (P : forall s, term s -> term s -> Prop)
-  (Hbeta : forall s x ty ty' body body' arg arg' args args',
-    pred1 ty ty' -> P s ty ty' ->
-    pred1 body body' -> P (s ▷ x) body body' ->
-    pred1 arg arg' -> P s arg arg' ->
-    All2 pred1 args args' -> All2 (P s) args args' ->
-    P s (TApp (TLam x ty body) (arg :: args)) (TApp (body'[x := arg']) args'))
-  (Htype : forall s, P s TType TType)
-  (Hvar : forall s i, P s (TVar i) (TVar i))
-  (Hlam : forall s x ty ty' body body',
-    pred1 ty ty' -> P s ty ty' ->
-    pred1 body body' -> P (s ▷ x) body body' ->
-    P s (TLam x ty body) (TLam x ty' body'))
-  (Hprod : forall s x a a' b b',
-    pred1 a a' -> P s a a' ->
-    pred1 b b' -> P (s ▷ x) b b' ->
-    P s (TProd x a b) (TProd x a' b'))
-  (Happ : forall s f f' args args',
-    pred1 f f' -> P s f f' ->
-    All2 pred1 args args' -> All2 (P s) args args' ->
-    P s (TApp f args) (TApp f' args'))
-  (Hevar : forall s ev, P s (TEvar ev) (TEvar ev)) :
-  forall s t t', pred1 t t' -> P s t t'.
+Lemma pred1_ind (P : forall s, evar_map -> term s -> term s -> Prop)
+  (Hbeta : forall s Σ x ty body body' arg arg' args args',
+    Σ |- body >> body' -> P (s ▷ x) Σ body body' ->
+    Σ |- arg >> arg' -> P s Σ arg arg' ->
+    All2 (pred1 Σ) args args' -> All2 (P s Σ) args args' ->
+    P s Σ (TApp (TLam x ty body) (arg :: args)) (TApp (body'[x := arg']) args'))
+  (Hexpand : forall s Σ ev ty def,
+    Σ ev = Some (mk_evar_entry ty (Some def)) ->
+    P s Σ (TEvar ev) (wk def))
+  (Htype : forall s Σ,
+    P s Σ TType TType)
+  (Hvar : forall s Σ i,
+    P s Σ (TVar i) (TVar i))
+  (Hlam : forall s Σ x ty ty' body body',
+    Σ |- ty >> ty' -> P s Σ ty ty' ->
+    Σ |- body >> body' -> P (s ▷ x) Σ body body' ->
+    P s Σ (TLam x ty body) (TLam x ty' body'))
+  (Hprod : forall s Σ x a a' b b',
+    Σ |- a >> a' -> P s Σ a a' ->
+    Σ |- b >> b' -> P (s ▷ x) Σ b b' ->
+    P s Σ (TProd x a b) (TProd x a' b'))
+  (Happ : forall s Σ f f' args args',
+    Σ |- f >> f' -> P s Σ f f' ->
+    All2 (pred1 Σ) args args' -> All2 (P s Σ) args args' ->
+    P s Σ (TApp f args) (TApp f' args'))
+  (Hevar : forall s Σ ev,
+    P s Σ (TEvar ev) (TEvar ev)) :
+  forall s Σ t t', Σ |- t >> t' -> P s Σ t t'.
 Proof.
-fix IH 4. intros s t t' Hred. destruct Hred.
-- apply Hbeta with ty' ; try assumption ; try now apply IH.
+fix IH 5. intros s Σ t t' Hred. destruct Hred.
+- apply Hbeta ; try assumption ; try now apply IH.
   revert args args' H. fix IHargs 3. intros args args' H. destruct H.
   + constructor.
   + constructor ; auto.
+- apply Hexpand with ty. assumption.
 - apply Htype.
 - apply Hvar.
 - apply Hlam ; auto.
@@ -86,32 +107,45 @@ fix IH 4. intros s t t' Hred. destruct Hred.
 - apply Hevar.
 Qed.
 
-#[export] Instance pred1_Reflexive s : Reflexive (@pred1 s).
+#[export] Instance pred1_Reflexive s Σ :
+  Reflexive (@pred1 s Σ).
 Proof.
 intros t. induction t using term_ind' ; constructor ; try assumption.
 induction args ; constructor ; depelim H ; auto.
 Qed.
 
-Lemma pred1_beta {s} x (ty : term s) body arg args :
-  pred1 (TApp (TLam x ty body) (arg :: args)) (TApp (body[x := arg]) args).
-Proof.
-eapply pred1_app_beta.
-- reflexivity.
-- reflexivity.
-- reflexivity.
-- now apply All2_same.
-Qed.
+(** Parallel reduction on substitutions is just pointwise parallel reduction. *)
+Definition pred1_subst {s s'} Σ (σ σ' : subst s s') : Prop :=
+  forall i, Σ |- sapply σ i >> sapply σ' i.
+
+Notation "Σ |- σ1 >>ₛ σ2" := (pred1_subst Σ σ1 σ2)
+  (at level 50, no associativity, σ1 at next level, σ2 at next level).
+
+#[export] Instance pred1_subst_Reflexive s s' Σ :
+  Reflexive (@pred1_subst s s' Σ).
+Proof. intros σ i. reflexivity. Qed.
 
 (***********************************************************************)
 (** * Relating parallel reduction and standard reduction. *)
 (***********************************************************************)
 
+(** [pred1] admits the beta rule. *)
+Lemma pred1_beta {s} Σ x (ty : term s) body arg args :
+  Σ |- TApp (TLam x ty body) (arg :: args) >> TApp (body[x := arg]) args.
+Proof.
+apply pred1_app_beta.
+- reflexivity.
+- reflexivity.
+- now apply All2_same.
+Qed.
+
 (** One-step reduction is included in parallel reduction. *)
-Lemma pred1_of_red1 {s} (t u : term s) :
-  red1 t u -> pred1 t u.
+Lemma pred1_of_red1 {s} Σ (t u : term s) :
+  Σ |- t ~>₁ u -> Σ |- t >> u.
 Proof.
 intros H. induction H.
 - apply pred1_beta.
+- eapply pred1_evar_expand ; eassumption.
 - now apply pred1_lam.
 - now apply pred1_lam.
 - now apply pred1_prod.
@@ -122,12 +156,14 @@ intros H. induction H.
 Qed.
 
 (** Parallel reduction is included in standard reduction. *)
-Lemma red_of_pred1 {s} (t u : term s) :
-  pred1 t u -> red t u.
+Lemma red_of_pred1 {s} Σ (t u : term s) :
+  Σ |- t >> u -> Σ |- t ~> u.
 Proof.
 intros H. induction H.
-- rewrite <-red_beta.
-  apply red_app_congr ; [apply red_lam_congr | constructor] ; eassumption.
+- rewrite <-red_beta. apply red_app_congr.
+  + now apply red_lam_congr.
+  + now constructor.
+- eapply red_evar_expand ; eassumption.
 - reflexivity.
 - reflexivity.
 - now apply red_lam_congr.
@@ -137,8 +173,8 @@ intros H. induction H.
 Qed.
 
 (** The reflexive closure of [pred1] is equal to [red]. *)
-Lemma red_is_pred {s} (t u : term s) :
-  red t u <-> refl_trans_clos pred1 t u.
+Lemma red_is_pred {s} Σ (t u : term s) :
+  Σ |- t ~> u <-> refl_trans_clos (pred1 Σ) t u.
 Proof.
 split ; revert t u ; apply refl_trans_clos_incl.
 - intros t u H. apply refl_trans_clos_one. now apply pred1_of_red1.
@@ -150,8 +186,8 @@ Qed.
 (***********************************************************************)
 
 (** Renaming lemma for [pred1]. *)
-Lemma pred1_rename {s s'} (t t' : term s) (ρ : ren s s') :
-  pred1 t t' -> pred1 (rename ρ t) (rename ρ t').
+Lemma pred1_rename {s s'} Σ (t t' : term s) (ρ : ren s s') :
+  Σ |- t >> t' -> Σ |- rename ρ t >> rename ρ t'.
 Proof.
 intros H. induction H in s', ρ |- * ; simpl_subst.
 - cbn.
@@ -159,7 +195,8 @@ intros H. induction H in s', ρ |- * ; simpl_subst.
           substitute (scons x (rename ρ arg') sid) (rename (rup x ρ) body')) as ->.
   { simpl_subst. f_equal. subst_ext i. depelim i ; simpl_subst ; reflexivity. }
   eapply pred1_app_beta ; eauto.
-  rewrite All2_map. revert H3. apply All2_consequence. firstorder.
+  rewrite All2_map. revert H2. apply All2_consequence. firstorder.
+- econstructor ; eassumption.
 - reflexivity.
 - reflexivity.
 - now apply pred1_lam.
@@ -170,19 +207,15 @@ intros H. induction H in s', ρ |- * ; simpl_subst.
 - reflexivity.
 Qed.
 
-(** Parallel reduction on substitutions is just pointwise parallel reduction. *)
-Definition pred1_subst {s s'} (σ σ' : subst s s') : Prop :=
-  forall i, pred1 (sapply σ i) (sapply σ' i).
-
-#[export] Instance pred1_subst_Reflexive s s' : Reflexive (@pred1_subst s s').
-Proof. intros σ i. reflexivity. Qed.
-
-Lemma pred1_subst_scons {x s s'} t t' (σ σ' : subst s s') :
-  pred1 t t' -> pred1_subst σ σ' -> pred1_subst (scons x t σ) (scons x t' σ').
+Lemma pred1_scons {x s s'} Σ t t' (σ σ' : subst s s') :
+  Σ |- t >> t' ->
+  Σ |- σ >>ₛ σ' ->
+  Σ |- scons x t σ >>ₛ scons x t' σ'.
 Proof. intros Ht Hσ i. depelim i ; simpl_subst ; auto. Qed.
 
-Lemma pred1_subst_sup {x s s'} (σ σ' : subst s s') :
-  pred1_subst σ σ' -> pred1_subst (sup x σ) (sup x σ').
+Lemma pred1_sup {x s s'} Σ (σ σ' : subst s s') :
+  Σ |- σ >>ₛ σ' ->
+  Σ |- sup x σ >>ₛ sup x σ'.
 Proof.
 intros H i. depelim i ; simpl_subst.
 - reflexivity.
@@ -190,10 +223,10 @@ intros H i. depelim i ; simpl_subst.
 Qed.
 
 (** Substitution lemma for [pred1]. *)
-Lemma pred1_substitute {s s'} (t t' : term s) (σ σ' : subst s s') :
-  pred1 t t' ->
-  pred1_subst σ σ' ->
-  pred1 (substitute σ t) (substitute σ' t').
+Lemma pred1_substitute {s s'} Σ (t t' : term s) (σ σ' : subst s s') :
+  Σ |- t >> t' ->
+  Σ |- σ >>ₛ σ' ->
+  Σ |- substitute σ t >> substitute σ' t'.
 Proof.
 intros Ht Hσ. induction Ht in s', σ, σ', Hσ |- * ; simpl_subst.
 - cbn.
@@ -201,12 +234,13 @@ intros Ht Hσ. induction Ht in s', σ, σ', Hσ |- * ; simpl_subst.
           substitute (scons x (substitute σ' arg') sid) (substitute (sup x σ') body')) as ->.
   { simpl_subst. f_equal. subst_ext i. depelim i ; simpl_subst ; reflexivity. }
   eapply pred1_app_beta ; eauto.
-  + apply IHHt2. now apply pred1_subst_sup.
+  + apply IHHt1. now apply pred1_sup.
   + rewrite All2_map. revert H0. apply All2_consequence. firstorder.
+- econstructor ; eauto.
 - reflexivity.
 - apply Hσ.
-- apply pred1_lam ; auto. apply IHHt2. now apply pred1_subst_sup.
-- apply pred1_prod ; auto. apply IHHt2. now apply pred1_subst_sup.
+- apply pred1_lam ; auto. apply IHHt2. now apply pred1_sup.
+- apply pred1_prod ; auto. apply IHHt2. now apply pred1_sup.
 - apply pred1_app ; auto. rewrite All2_map. revert H0.
   apply All2_consequence. firstorder.
 - reflexivity.
@@ -217,64 +251,68 @@ Qed.
 (***********************************************************************)
 
 (** Two terms are joinable if they have a common reduct for [pred1]. *)
-Definition joinable {s} (t1 t2 : term s) : Prop :=
-  exists u, pred1 t1 u /\ pred1 t2 u.
+Definition joinable {s} Σ (t1 t2 : term s) : Prop :=
+  exists u, Σ |- t1 >> u /\ Σ |- t2 >> u.
 
-#[export] Instance joinable_Reflexive s : Reflexive (@joinable s).
+#[export] Instance joinable_Reflexive s Σ :
+  Reflexive (@joinable s Σ).
 Proof. intros t. exists t. now split. Qed.
 
-#[export] Instance joinable_Symmetric s : Symmetric (@joinable s).
+#[export] Instance joinable_Symmetric s Σ :
+  Symmetric (@joinable s Σ).
 Proof. intros t1 t2. unfold joinable. firstorder. Qed.
 
 (** Two substitutions are joinable if they are pointwise joinable. *)
-Definition joinable_subst {s s'} (σ1 σ2 : subst s s') : Prop :=
-  exists σ, pred1_subst σ1 σ /\ pred1_subst σ2 σ.
+Definition joinable_subst {s s'} Σ (σ1 σ2 : subst s s') : Prop :=
+  exists σ, Σ |- σ1 >>ₛ σ /\ Σ |- σ2 >>ₛ σ.
 
-#[export] Instance joinable_subst_Reflexive s s' : Reflexive (@joinable_subst s s').
+#[export] Instance joinable_subst_Reflexive s s' Σ :
+  Reflexive (@joinable_subst s s' Σ).
 Proof. intros σ. exists σ. split ; reflexivity. Qed.
 
-#[export] Instance joinable_subst_Symmetric s s' : Symmetric (@joinable_subst s s').
+#[export] Instance joinable_subst_Symmetric s s' Σ :
+  Symmetric (@joinable_subst s s' Σ).
 Proof. intros σ1 σ2 (σ & H1 & H2). exists σ. firstorder. Qed.
 
-Lemma joinable_scons {x s s'} t1 t2 (σ1 σ2 : subst s s') :
-  joinable t1 t2 ->
-  joinable_subst σ1 σ2 ->
-  joinable_subst (scons x t1 σ1) (scons x t2 σ2).
+Lemma joinable_scons {x s s'} Σ t1 t2 (σ1 σ2 : subst s s') :
+  joinable Σ t1 t2 ->
+  joinable_subst Σ σ1 σ2 ->
+  joinable_subst Σ (scons x t1 σ1) (scons x t2 σ2).
 Proof.
 intros (t & Ht1 & Ht2) (σ & Hσ1 & Hσ2). exists (scons x t σ).
-split ; now apply pred1_subst_scons.
+split ; now apply pred1_scons.
 Qed.
 
-Lemma joinable_substitute {s s'} (t1 t2 : term s) (σ1 σ2 : subst s s') :
-  joinable t1 t2 ->
-  joinable_subst σ1 σ2 ->
-  joinable (substitute σ1 t1) (substitute σ2 t2).
+Lemma joinable_substitute {s s'} Σ (t1 t2 : term s) (σ1 σ2 : subst s s') :
+  joinable Σ t1 t2 ->
+  joinable_subst Σ σ1 σ2 ->
+  joinable Σ (substitute σ1 t1) (substitute σ2 t2).
 Proof.
 intros (t & Ht1 & Ht2) (σ & Hσ1 & Hσ2). exists (substitute σ t).
 split ; now apply pred1_substitute.
 Qed.
 
-Lemma joinable_lam {s x} (ty1 ty2 : term s) body1 body2 :
-  joinable ty1 ty2 ->
-  joinable body1 body2 ->
-  joinable (TLam x ty1 body1) (TLam x ty2 body2).
+Lemma joinable_lam {s x} Σ (ty1 ty2 : term s) body1 body2 :
+  joinable Σ ty1 ty2 ->
+  joinable Σ body1 body2 ->
+  joinable Σ (TLam x ty1 body1) (TLam x ty2 body2).
 Proof.
 intros (ty & Hty1 & Hty2) (body & Hbody1 & Hbody2).
 exists (TLam x ty body). split ; apply pred1_lam ; assumption.
 Qed.
 
-Lemma joinable_prod {s x} (a1 a2 : term s) b1 b2 :
-  joinable a1 a2 ->
-  joinable b1 b2 ->
-  joinable (TProd x a1 b1) (TProd x a2 b2).
+Lemma joinable_prod {s x} Σ (a1 a2 : term s) b1 b2 :
+  joinable Σ a1 a2 ->
+  joinable Σ b1 b2 ->
+  joinable Σ (TProd x a1 b1) (TProd x a2 b2).
 Proof.
 intros (a & Ha1 & Ha2) (b & Hb1 & Hb2).
 exists (TProd x a b). split ; apply pred1_prod ; assumption.
 Qed.
 
-Lemma joinable_list {s} (args1 args2 : list (term s)) :
-  All2 joinable args1 args2 ->
-  exists args, All2 pred1 args1 args /\ All2 pred1 args2 args.
+Lemma joinable_list {s} Σ (args1 args2 : list (term s)) :
+  All2 (joinable Σ) args1 args2 ->
+  exists args, All2 (pred1 Σ) args1 args /\ All2 (pred1 Σ) args2 args.
 Proof.
 intros H. induction H.
 - exists []. split ; constructor.
@@ -282,28 +320,27 @@ intros H. induction H.
   exists (z :: args). split ; constructor ; assumption.
 Qed.
 
-Lemma joinable_app {s} (f1 f2 : term s) args1 args2 :
-  joinable f1 f2 ->
-  All2 joinable args1 args2 ->
-  joinable (TApp f1 args1) (TApp f2 args2).
+Lemma joinable_app {s} Σ (f1 f2 : term s) args1 args2 :
+  joinable Σ f1 f2 ->
+  All2 (joinable Σ) args1 args2 ->
+  joinable Σ (TApp f1 args1) (TApp f2 args2).
 Proof.
 intros (f & Hf1 & Hf2) Hargs. apply joinable_list in Hargs.
 destruct Hargs as (args & Hargs1 & Hargs2).
 exists (TApp f args). split ; apply pred1_app ; assumption.
 Qed.
 
-Lemma joinable_beta {s x} (ty1 ty2 : term s) body1 body2 (arg1 arg2 : term s) args1 args2 :
-  joinable ty1 ty2 ->
-  joinable body1 body2 ->
-  joinable arg1 arg2 ->
-  All2 joinable args1 args2 ->
-  joinable (TApp (body1[x := arg1]) args1) (TApp (TLam x ty2 body2) (arg2 :: args2)).
+Lemma joinable_beta {s x} Σ ty2 body1 body2 (arg1 arg2 : term s) args1 args2 :
+  joinable Σ body1 body2 ->
+  joinable Σ arg1 arg2 ->
+  All2 (joinable Σ) args1 args2 ->
+  joinable Σ (TApp (body1[x := arg1]) args1) (TApp (TLam x ty2 body2) (arg2 :: args2)).
 Proof.
-intros (ty & Hty1 & Hty2) (body & Hbody1 & Hbody2) (arg & Harg1 & Harg2) Hargs.
+intros (body & Hbody1 & Hbody2) (arg & Harg1 & Harg2) Hargs.
 apply joinable_list in Hargs. destruct Hargs as (args & Hargs1 & Hargs2).
 exists (TApp (body[x := arg]) args). split.
 - apply pred1_app.
-  + apply pred1_substitute ; [| apply pred1_subst_scons].
+  + apply pred1_substitute ; [| apply pred1_scons].
     * assumption.
     * assumption.
     * reflexivity.
@@ -326,37 +363,38 @@ intros H HP HQ. revert zs HQ. depind HP ; intros zs HQ ; depelim HQ ; constructo
 Qed.
 
 (** [pred1] has the diamond property. *)
-Lemma pred1_diamond {s} (t u1 u2 : term s) :
-  pred1 t u1 -> pred1 t u2 -> joinable u1 u2.
+Lemma pred1_diamond {s} Σ (t u1 u2 : term s) :
+  Σ |- t >> u1 -> Σ |- t >> u2 -> joinable Σ u1 u2.
 Proof.
 intros H1 H2. depind H1 ; depelim H2 ; try reflexivity.
 - apply joinable_app ; [apply joinable_substitute ; [| apply joinable_scons] |].
+  + now apply IHpred1_1.
   + now apply IHpred1_2.
-  + now apply IHpred1_3.
   + reflexivity.
   + revert H0 H1. apply All2_weird_consequence. firstorder.
 - depelim H2. depelim H1. eapply joinable_beta.
   + now apply IHpred1_1.
   + now apply IHpred1_2.
-  + now apply IHpred1_3.
   + revert H0 H2. apply All2_weird_consequence. firstorder.
+- rewrite H in H0. depelim H0. reflexivity.
+- exists (wk def). split ; [reflexivity |]. econstructor ; eassumption.
 - apply joinable_lam ; auto.
 - apply joinable_prod ; auto.
 - depelim H1. depelim H. depelim H1.
-  specialize (IHpred1 (TLam x ty'0 body')). feed IHpred1. { now apply pred1_lam. }
+  specialize (IHpred1 (TLam x ty' body')). feed IHpred1. { now apply pred1_lam. }
   destruct IHpred1 as (z & Hz1 & Hz2). depelim Hz1. depelim Hz2.
   apply inj_right_sigma in H3. depelim H3.
   symmetry. eapply joinable_beta.
   + eexists ; eauto.
-  + eexists ; eauto.
   + symmetry. auto.
   + revert H4 H2. apply All2_weird_consequence. firstorder.
 - apply joinable_app ; auto. revert H0 H3. apply All2_weird_consequence. firstorder.
+- exists (wk def). split ; [|reflexivity]. econstructor ; eassumption.
 Qed.
 
 (** [pred1] is confluent. This is a consequence of the diamond property. *)
-Lemma pred1_confluence {s} :
-  diamond (refl_trans_clos (@pred1 s)) (refl_trans_clos (@pred1 s)).
+Lemma pred1_confluence {s} Σ :
+  diamond (refl_trans_clos (@pred1 s Σ)) (refl_trans_clos (@pred1 s Σ)).
 Proof. apply diamond_confluence. intros t u1 u2. apply pred1_diamond. Qed.
 
 (***********************************************************************)
@@ -364,12 +402,12 @@ Proof. apply diamond_confluence. intros t u1 u2. apply pred1_diamond. Qed.
 (***********************************************************************)
 
 (** Confluence for [red] is an immediate result of the confluence for [pred1]. *)
-Lemma red_confluence {s} (t u1 u2 : term s) :
-  red t u1 ->
-  red t u2 ->
-  exists v, red u1 v /\ red u2 v.
+Lemma red_confluence {s} Σ (t u1 u2 : term s) :
+  Σ |- t ~> u1 ->
+  Σ |- t ~> u2 ->
+  exists v, Σ |- u1 ~> v /\ Σ |- u2 ~> v.
 Proof.
 intros H1 H2. rewrite red_is_pred in H1, H2.
-pose proof (H := pred1_confluence t u1 u2 H1 H2).
+pose proof (H := pred1_confluence Σ t u1 u2 H1 H2).
 destruct H as (v & Hv1 & Hv2). exists v. rewrite !red_is_pred. now split.
 Qed.
