theories/MetaTheory/Reduction.v
@@ -1,5 +1,5 @@
 From Metaprog Require Import Prelude.
-From Metaprog.MetaTheory Require Export Relations Substitution.
+From Metaprog.MetaTheory Require Export Relations Substitution EvarMap.
 
 (** This module defines:
     - The one-step strong reduction relation [red1] on [term].
@@ -9,32 +9,42 @@ From Metaprog.MetaTheory Require Export Relations Substitution.
 (** * One-step reduction relation [red1]. *)
 (***********************************************************************)
 
+Reserved Notation "Σ |- t ~>₁ u"
+  (at level 50, no associativity, t at next level, u at next level).
+
 Unset Elimination Schemes.
 
 (** Strong one-step reduction relation. This relation is _not_ deterministic. *)
-Inductive red1 {s} : term s -> term s -> Prop :=
+Inductive red1 {s} Σ : term s -> term s -> Prop :=
 
 (** Beta-reduction rule. *)
 | red1_beta x ty body arg args :
-    red1 (TApp (TLam x ty body) (arg :: args)) (TApp (body[x := arg]) args)
+    Σ |- TApp (TLam x ty body) (arg :: args) ~>₁ TApp (body[x := arg]) args
+
+(** Evar expansion. *)
+| red1_evar_expand ev ty def :
+    Σ ev = Some (mk_evar_entry ty (Some def)) ->
+    Σ |- TEvar ev ~>₁ wk def
 
 (** Congrence rules for [TLam]. *)
 | red1_lam_l x ty ty' body :
-    red1 ty ty' -> red1 (TLam x ty body) (TLam x ty' body)
+    Σ |- ty ~>₁ ty' -> Σ |- TLam x ty body ~>₁ TLam x ty' body
 | red1_lam_r x ty body body' :
-    red1 body body' -> red1 (TLam x ty body) (TLam x ty body')
+    Σ |- body ~>₁ body' -> Σ |- TLam x ty body ~>₁ TLam x ty body'
 
 (** Congruence rules for [TProd]. *)
 | red1_prod_l x a a' b :
-    red1 a a' -> red1 (TProd x a b) (TProd x a' b)
+    Σ |- a ~>₁ a' -> Σ |- TProd x a b ~>₁ TProd x a' b
 | red1_prod_r x a b b' :
-    red1 b b' -> red1 (TProd x a b) (TProd x a b')
+    Σ |- b ~>₁ b' -> Σ |- TProd x a b ~>₁ TProd x a b'
 
 (** Congruence rules for [TApp]. *)
 | red1_app_l f f' args :
-    red1 f f' -> red1 (TApp f args) (TApp f' args)
+    Σ |- f ~>₁ f' -> Σ |- TApp f args ~>₁ TApp f' args
 | red1_app_r f args args' :
-    OnOne2 red1 args args' -> red1 (TApp f args) (TApp f args').
+    OnOne2 (red1 Σ) args args' -> Σ |- TApp f args ~>₁ TApp f args'
+
+where "Σ |- t ~>₁ u" := (red1 Σ t u).
 
 Set Elimination Schemes.
 
@@ -42,37 +52,41 @@ Derive Signature for red1.
 
 (** Induction principle for [red1]. We can't use Rocq's default induction principle
     because [red1] is nested over [OnOne2]. *)
-Lemma red1_ind (P : forall s, term s -> term s -> Prop) :
-  (forall s x ty body arg args,
-    P s (TApp (TLam x ty body) (arg :: args)) (TApp (body[x := arg]) args)) ->
-  (forall s x ty ty' body,
-    red1 ty ty' ->
-    P s ty ty' ->
-    P s (TLam x ty body) (TLam x ty' body)) ->
-  (forall s x ty body body',
-    red1 body body' ->
-    P (s ▷ x) body body' ->
-    P s (TLam x ty body) (TLam x ty body')) ->
-  (forall s x a a' b,
-    red1 a a' ->
-    P s a a' ->
-    P s (TProd x a b) (TProd x a' b)) ->
-  (forall s x a b b',
-    red1 b b' ->
-    P (s ▷ x) b b' ->
-    P s (TProd x a b) (TProd x a b')) ->
-  (forall s f f' args,
-    red1 f f' ->
-    P s f f' ->
-    P s (TApp f args) (TApp f' args)) ->
-  (forall s f args args',
-    OnOne2 (fun arg arg' => red1 arg arg' /\ P s arg arg') args args' ->
-    P s (TApp f args) (TApp f args')) ->
-  forall s t t', red1 t t' -> P s t t'.
+Lemma red1_ind (P : forall s, evar_map -> term s -> term s -> Prop) :
+  (forall s Σ x ty body arg args,
+    P s Σ (TApp (TLam x ty body) (arg :: args)) (TApp (body[x := arg]) args)) ->
+  (forall s Σ ev ty def,
+    Σ ev = Some (mk_evar_entry ty (Some def)) ->
+    P s Σ (TEvar ev) (wk def)) ->
+  (forall s Σ x ty ty' body,
+    Σ |- ty ~>₁ ty' ->
+    P s Σ ty ty' ->
+    P s Σ (TLam x ty body) (TLam x ty' body)) ->
+  (forall s Σ x ty body body',
+    Σ |- body ~>₁ body' ->
+    P (s ▷ x) Σ body body' ->
+    P s Σ (TLam x ty body) (TLam x ty body')) ->
+  (forall s Σ x a a' b,
+    Σ |- a ~>₁ a' ->
+    P s Σ a a' ->
+    P s Σ (TProd x a b) (TProd x a' b)) ->
+  (forall s Σ x a b b',
+    Σ |- b ~>₁ b' ->
+    P (s ▷ x) Σ b b' ->
+    P s Σ (TProd x a b) (TProd x a b')) ->
+  (forall s Σ f f' args,
+    Σ |- f ~>₁ f' ->
+    P s Σ f f' ->
+    P s Σ (TApp f args) (TApp f' args)) ->
+  (forall s Σ f args args',
+    OnOne2 (fun arg arg' => Σ |- arg ~>₁ arg' /\ P s Σ arg arg') args args' ->
+    P s Σ (TApp f args) (TApp f args')) ->
+  forall s Σ t t', Σ |- t ~>₁ t' -> P s Σ t t'.
 Proof.
-intros Hbeta Hlam_l Hlam_r Hprod_l Hprod_r Happ_l Happ_r. fix IH 4.
-intros s t t' Hred. destruct Hred.
+intros Hbeta Hevar Hlam_l Hlam_r Hprod_l Hprod_r Happ_l Happ_r. fix IH 5.
+intros s Σ t t' Hred. destruct Hred.
 - apply Hbeta.
+- eapply Hevar. eassumption.
 - apply Hlam_l ; auto.
 - apply Hlam_r ; auto.
 - apply Hprod_l ; auto.
@@ -88,17 +102,20 @@ Qed.
 (***********************************************************************)
 
 (** Strong reduction relation, defined as the reflexive-transitive closure of [red1]. *)
-Definition red {s} : term s -> term s -> Prop :=
-  refl_trans_clos (@red1 s).
+Definition red {s} (Σ : evar_map) : term s -> term s -> Prop :=
+  refl_trans_clos (@red1 s Σ).
 
 Arguments red : simpl never.
 
-Lemma red_same {s} (t u : term s) :
-  t = u -> red t u.
+Notation "Σ |- t ~> u" := (red Σ t u)
+  (at level 50, no associativity, t at next level, u at next level).
+
+Lemma red_same {s} Σ (t u : term s) :
+  t = u -> Σ |- t ~> u.
 Proof. intros ->. reflexivity. Qed.
 
-Lemma red_of_red1 {s} (t u : term s) :
-  red1 t u -> red t u.
+Lemma red_of_red1 {s} Σ (t u : term s) :
+  Σ |- t ~>₁ u -> Σ |- t ~> u.
 Proof. apply refl_trans_clos_one. Qed.
 
 (***********************************************************************)
@@ -106,16 +123,21 @@ Proof. apply refl_trans_clos_one. Qed.
 (***********************************************************************)
 
 Section CongruenceLemmas.
-  Context {s : scope}.
+  Context {s : scope} (Σ : evar_map).
 
   Lemma red_beta x (ty : term s) body arg args :
-    red (TApp (TLam x ty body) (arg :: args)) (TApp (body[x := arg]) args).
+    Σ |- TApp (TLam x ty body) (arg :: args) ~> TApp (body[x := arg]) args.
   Proof. apply red_of_red1. constructor. Qed.
 
+  Lemma red_evar_expand ev ty def :
+    Σ ev = Some (mk_evar_entry ty (Some def)) ->
+    Σ |- @TEvar s ev ~> wk def.
+  Proof. intros H. apply red_of_red1. econstructor ; eauto. Qed.
+
   Lemma red_lam_congr x (ty ty' : term s) body body' :
-    red ty ty' ->
-    red body body' ->
-    red (TLam x ty body) (TLam x ty' body').
+    Σ |- ty ~> ty' ->
+    Σ |- body ~> body' ->
+    Σ |- TLam x ty body ~> TLam x ty' body'.
   Proof.
   intros Hty Hbody. transitivity (TLam x ty body').
   - clear Hty. induction Hbody.
@@ -127,9 +149,9 @@ Section CongruenceLemmas.
   Qed.
 
   Lemma red_prod_congr x (a a' : term s) b b' :
-    red a a' ->
-    red b b' ->
-    red (TProd x a b) (TProd x a' b').
+    Σ |- a ~> a' ->
+    Σ |- b ~> b' ->
+    Σ |- TProd x a b ~> TProd x a' b'.
   Proof.
   intros Ha Hb. transitivity (TProd x a b').
   - clear Ha. induction Hb.
@@ -141,8 +163,8 @@ Section CongruenceLemmas.
   Qed.
 
   Lemma red_app_congr_aux (f : term s) l (args args' : list (term s)) :
-    All2 red args args' ->
-    red (TApp f (l ++ args)) (TApp f (l ++ args')).
+    All2 (red Σ) args args' ->
+    Σ |- TApp f (l ++ args) ~> TApp f (l ++ args').
   Proof.
   intros H. revert f l. depind H ; intros f l.
   - reflexivity.
@@ -156,9 +178,9 @@ Section CongruenceLemmas.
   Qed.
 
   Lemma red_app_congr (f f' : term s) args args' :
-    red f f' ->
-    All2 red args args' ->
-    red (TApp f args) (TApp f' args').
+    Σ |- f ~> f' ->
+    All2 (red Σ) args args' ->
+    Σ |- TApp f args ~> TApp f' args'.
   Proof.
   intros Hf Hargs. transitivity (TApp f' args).
   - clear Hargs. induction Hf.
@@ -174,10 +196,10 @@ End CongruenceLemmas.
 (***********************************************************************)
 
 Section InversionLemmas.
-  Context {s : scope}.
+  Context {s : scope} (Σ : evar_map).
 
   Lemma red_type_inv (t : term s) :
-    red TType t -> t = TType.
+    Σ |- TType ~> t -> t = TType.
   Proof.
   intros H. depind H.
   - reflexivity.
@@ -185,7 +207,7 @@ Section InversionLemmas.
   Qed.
 
   Lemma red_var_inv (i : index s) (t : term s) :
-    red (TVar i) t -> t = TVar i.
+    Σ |- TVar i ~> t -> t = TVar i.
   Proof.
   intros H. depind H.
   - reflexivity.
@@ -193,11 +215,11 @@ Section InversionLemmas.
   Qed.
 
   Lemma red_lam_inv x (ty : term s) body t :
-    red (TLam x ty body) t ->
+    Σ |- TLam x ty body ~> t ->
     exists ty' body',
       t = TLam x ty' body' /\
-      red ty ty' /\
-      red body body'.
+      Σ |- ty ~> ty' /\
+      Σ |- body ~> body'.
   Proof.
   intros Hred. depind Hred.
   - exists ty, body. now split3.
@@ -209,11 +231,11 @@ Section InversionLemmas.
   Qed.
 
   Lemma red_prod_inv x (a : term s) b t :
-    red (TProd x a b) t ->
+    Σ |- TProd x a b ~> t ->
     exists a' b',
       t = TProd x a' b' /\
-      red a a' /\
-      red b b'.
+      Σ |- a ~> a' /\
+      Σ |- b ~> b'.
   Proof.
   intros Hred. depind Hred.
   - exists a, b. now split3.
@@ -224,13 +246,13 @@ Section InversionLemmas.
       rewrite Hb1. now apply red_of_red1.
   Qed.
 
-  Lemma red_evar_inv ev (t : term s) :
+  (*Lemma red_evar_inv ev (t : term s) :
     red (TEvar ev) t -> t = TEvar ev.
   Proof.
   intros H. depind H.
   - reflexivity.
   - subst. depelim H0.
-  Qed.
+  Qed.*)
 
 End InversionLemmas.
 
@@ -239,11 +261,11 @@ End InversionLemmas.
 (***********************************************************************)
 
 Section SubstitutionLemma.
-  Context {s s' : scope}.
+  Context {s s' : scope} (Σ : evar_map).
 
   (** Renaming lemma for [red1]. *)
   Lemma red1_rename (t t' : term s) (ρ : ren s s') :
-    red1 t t' -> red1 (rename ρ t) (rename ρ t').
+    Σ |- t ~>₁ t' -> Σ |- rename ρ t ~>₁ rename ρ t'.
   Proof.
   intros H. induction H in s', ρ |- * ; simpl_subst.
   - cbn.
@@ -251,6 +273,7 @@ Section SubstitutionLemma.
             substitute (scons x (rename ρ arg) sid) (rename (rup x ρ) body)) as ->.
     { simpl_subst. f_equal. subst_ext i. depelim i ; simpl_subst ; reflexivity. }
     apply red1_beta.
+  - eapply red1_evar_expand. eassumption.
   - now apply red1_lam_l.
   - now apply red1_lam_r.
   - now apply red1_prod_l.
@@ -261,7 +284,7 @@ Section SubstitutionLemma.
 
   (** Renaming lemma for [red]. *)
   Lemma red_rename (t t' : term s) (ρ : ren s s') :
-    red t t' -> red (rename ρ t) (rename ρ t').
+    Σ |- t ~> t' -> Σ |- rename ρ t ~> rename ρ t'.
   Proof.
   intros H. induction H.
   - reflexivity.
@@ -270,7 +293,7 @@ Section SubstitutionLemma.
 
   (** Substitution lemma for [red1]. *)
   Lemma red1_substitute (t t' : term s) (σ : subst s s') :
-    red1 t t' -> red1 (substitute σ t) (substitute σ t').
+    Σ |- t ~>₁ t' -> Σ |- substitute σ t ~>₁ substitute σ t'.
   Proof.
   intros H. induction H in s', σ |- * ; simpl_subst.
   - cbn.
@@ -278,6 +301,7 @@ Section SubstitutionLemma.
             substitute (scons x (substitute σ arg) sid) (substitute (sup x σ) body)) as ->.
     { simpl_subst. f_equal. subst_ext i. depelim i ; simpl_subst ; reflexivity. }
     apply red1_beta.
+  - eapply red1_evar_expand. eassumption.
   - now apply red1_lam_l.
   - now apply red1_lam_r.
   - now apply red1_prod_l.
@@ -288,7 +312,7 @@ Section SubstitutionLemma.
 
   (** Substitution lemma for [red]. *)
   Lemma red_substitute (t t' : term s) (σ : subst s s') :
-    red t t' -> red (substitute σ t) (substitute σ t').
+    Σ |- t ~> t' -> Σ |- substitute σ t ~> substitute σ t'.
   Proof.
   intros H. induction H.
   - reflexivity.
